Status as of 1679334468

ch7/IMP.thy
@@ -4,7 +4,8 @@ begin
 
 (* Data type definitions *)
 
-(* Arithmetic expression (i.e. aexp) primitives from 3.1.1 *)
+(* Arithmetic expression (i.e. aexp) primitives from
+   3.1.1 *)
 type_synonym vname = string
 datatype aexp =
   N int
@@ -22,7 +23,8 @@ datatype bexp =
   | And bexp bexp
   | Less aexp aexp
 
-(* IMP language command (i.e. com) specification from 7.1 *)
+(* IMP language command (i.e. com) specification from
+   7.1 *)
 datatype com =
   SKIP
   | Assign vname aexp ("_ ::= _")
@@ -33,188 +35,219 @@ datatype com =
 
 (* Convenient helpers *)
 fun Or :: "bexp \<Rightarrow> bexp \<Rightarrow> bexp" where
-"Or a b = (Not (And (Not a) (Not b)))"
+    "Or a b = (Not (And (Not a) (Not b)))"
 
 fun Cond :: "bexp \<Rightarrow> bexp \<Rightarrow> bexp" where
-"Cond a b = (Or (Not a) b)"
+    "Cond a b = (Or (Not a) b)"
 
 fun VarEq :: "vname \<Rightarrow> aexp \<Rightarrow> bexp" where
-"VarEq x a = (And (Not (Less (V x) a)) (Not (Less a (V x))))"
+    "VarEq x a =
+      (And
+        (Not (Less (V x) a))
+        (Not (Less a (V x))))"
 
 (* Semantic definitions *)
 
 (* Arithmetic expression evaluation from 3.1.2 *)
 fun aval :: "aexp \<Rightarrow> state \<Rightarrow> val" where
-"aval (N n) s = n" |
-"aval (V x) s= s x" |
-"aval (Plus a1 a2) s = aval a1 s + aval a2 s"
+    "aval (N n) s = n" |
+    "aval (V x) s = s x" |
+    "aval (Plus a1 a2) s = aval a1 s + aval a2 s"
+
+lemma unequal_plus:
+    "n \<noteq> 0
+    \<Longrightarrow> aval (V x) s \<noteq> aval (Plus (V x) (N n)) s"
+  by simp
+
 
 (* Boolean expression evaluation from 3.2 *)
 fun bval :: "bexp \<Rightarrow> state \<Rightarrow> bool" where
-"bval (Bc v) s = v" |
-"bval (Not b) s = (\<not> bval b s)" |
-"bval (And b1 b2) s = (bval b1 s \<and> bval b2 s)" |
-"bval (Less a1 a2) s = (aval a1 s < aval a2 s)"
+    "bval (Bc v) s = v" |
+    "bval (Not b) s = (\<not> bval b s)" |
+    "bval (And b1 b2) s = (bval b1 s \<and> bval b2 s)" |
+    "bval (Less a1 a2) s = (aval a1 s < aval a2 s)"
 
 (* Big-step semantics for IMP from 7.2.1 *)
 inductive big_step :: "com \<times> state \<Rightarrow> state \<Rightarrow> bool"
   (infix "\<Rightarrow>" 55) where
 Skip: "(SKIP,s) \<Rightarrow> s" |
 Assign: "(x ::= a,s) \<Rightarrow> s(x := aval a s)" |
-Seq: "
-  \<lbrakk> (c1,s1) \<Rightarrow> s2; (c2,s2) \<Rightarrow> s3 \<rbrakk>
-  \<Longrightarrow> (c1;;c2,s1) \<Rightarrow> s3
-" |
-IfTrue: "
-  \<lbrakk> bval b s; (c1,s) \<Rightarrow>t \<rbrakk>
-  \<Longrightarrow> (IF b THEN c1 ELSE c2,s) \<Rightarrow> t
-" |
-IfFalse: "
-  \<lbrakk> \<not>bval b s; (c2,s) \<Rightarrow> t \<rbrakk>
-  \<Longrightarrow> (IF b THEN c1 ELSE c2,s) \<Rightarrow> t
-" |
-WhileFalse: "
-  \<not>bval b s
-  \<Longrightarrow> (WHILE b DO c,s) \<Rightarrow> s
-" |
-WhileTrue: "
-  \<lbrakk> bval b s1; (c,s1) \<Rightarrow> s2; (WHILE b DO c,s2) \<Rightarrow> s3 \<rbrakk>
-  \<Longrightarrow> (WHILE b DO c,s1) \<Rightarrow> s3
-"
+Seq:
+    "\<lbrakk> (c1,s1) \<Rightarrow> s2; (c2,s2) \<Rightarrow> s3 \<rbrakk>
+    \<Longrightarrow> (c1;;c2,s1) \<Rightarrow> s3" |
+IfTrue:
+    "\<lbrakk> bval b s; (c1,s) \<Rightarrow>t \<rbrakk>
+    \<Longrightarrow> (IF b THEN c1 ELSE c2,s) \<Rightarrow> t" |
+IfFalse:
+    "\<lbrakk> \<not>bval b s; (c2,s) \<Rightarrow> t \<rbrakk>
+    \<Longrightarrow> (IF b THEN c1 ELSE c2,s) \<Rightarrow> t" |
+WhileFalse:
+    "\<not>bval b s
+    \<Longrightarrow> (WHILE b DO c,s) \<Rightarrow> s" |
+WhileTrue:
+    "\<lbrakk> bval b s1; (c,s1) \<Rightarrow> s2; (WHILE b DO c,s2) \<Rightarrow> s3 \<rbrakk>
+    \<Longrightarrow> (WHILE b DO c,s1) \<Rightarrow> s3"
 
-(* Big step tweaks to simplify usage as found in
+(* Big-step tweaks to simplify usage as found in
    the implementation included in the Isabelle source *)
 declare big_step.intros [intro]
-lemmas big_step_induct = big_step.induct[split_format(complete)]
+lemmas big_step_induct =
+    big_step.induct[split_format(complete)]
 inductive_cases SkipE[elim!]: "(SKIP,s) \<Rightarrow> t"
 inductive_cases AssignE[elim!]: "(x ::= c,s) \<Rightarrow> t"
 inductive_cases SeqE[elim!]: "(c1 ;; c2,s) \<Rightarrow> t"
-inductive_cases IfE[elim!]: "(IF b THEN c1 ELSE c2,s) \<Rightarrow> t"
+inductive_cases IfE[elim!]:
+    "(IF b THEN c1 ELSE c2,s) \<Rightarrow> t"
 inductive_cases WhileE[elim]: "(WHILE b DO c,s) \<Rightarrow> t"
 
 (* Small-step semantic rules from 7.3 *)
-inductive small_step :: "com \<times> state \<Rightarrow> com \<times> state \<Rightarrow> bool"
+inductive small_step ::
+    "com \<times> state \<Rightarrow> com \<times> state \<Rightarrow> bool"
   (infix "\<rightarrow>" 55) where
 Assign: "(x ::= a,s) \<rightarrow> (SKIP,s(x := aval a s))" |
 Seq1: "(SKIP;;c2,s) \<rightarrow> (c2,s)" |
-Seq2: "(c1,s) \<rightarrow> (c1',s') \<Longrightarrow> (c1;;c2,s) \<rightarrow> (c1';;c2,s')" |
-IfTrue: "bval b s \<Longrightarrow> (IF b THEN c1 ELSE c2,s) \<rightarrow> (c1,s)" |
-IfFalse: "\<not>bval b s \<Longrightarrow> (IF b THEN c1 ELSE c2,s) \<rightarrow> (c2,s)" |
-While: "(WHILE b DO c,s) \<rightarrow> (IF b THEN c;;WHILE b DO c ELSE SKIP,s)"
+Seq2:
+    "(c1,s) \<rightarrow> (c1',s')
+    \<Longrightarrow> (c1;;c2,s) \<rightarrow> (c1';;c2,s')" |
+IfTrue:
+    "bval b s
+    \<Longrightarrow> (IF b THEN c1 ELSE c2,s) \<rightarrow> (c1,s)" |
+IfFalse:
+    "\<not>bval b s
+    \<Longrightarrow> (IF b THEN c1 ELSE c2,s) \<rightarrow> (c2,s)" |
+While:
+    "(WHILE b DO c,s)
+    \<rightarrow> (IF b THEN c;;WHILE b DO c ELSE SKIP,s)"
+
+(* Small-step tweaks *)
+lemmas small_step_induct =
+    small_step.induct[split_format(complete)]
+declare small_step.intros[intro,simp]
+inductive_cases SmallSkipE[elim!]: "(SKIP,s) \<rightarrow> ct"
+inductive_cases SmallAssignE[elim!]: "(x::=a,s) \<rightarrow> ct"
+inductive_cases SmallSeqE[elim]: "(c1;;c2,s) \<rightarrow> ct"
+inductive_cases SmallIfE[elim!]:
+    "(IF b THEN c1 ELSE c2,s) \<rightarrow> ct"
+inductive_cases SmallWhileE[elim]:
+    "(WHILE b DO c,s) \<rightarrow> ct"
+
 
 
 (* Semantic helpers *)
 
 (* Rule inversion equivalence lemmas from 7.2.3 *)
 lemma skip_state_equiv:
-  "(SKIP,s) \<Rightarrow> t \<longleftrightarrow> t = s" (is "?LHS \<longleftrightarrow> ?RHS")
+    "(SKIP,s) \<Rightarrow> t \<longleftrightarrow> t = s"
+  (is "?LHS \<longleftrightarrow> ?RHS")
 proof
-  assume "?LHS"
-  thus "?RHS" by cases
+  assume "?LHS" thus "?RHS" by cases
 next
-  assume "?RHS"
-  thus "?LHS" by (simp add: Skip)
+  assume "?RHS" thus "?LHS" by (simp add: Skip)
 qed
 
 lemma assign_state:
-  "(x ::= a,s) \<Rightarrow> t \<longleftrightarrow> t = s(x := aval a s)"
+    "(x ::= a,s) \<Rightarrow> t \<longleftrightarrow> t = s(x := aval a s)"
   (is "?LHS \<longleftrightarrow> ?RHS")
 proof
-  assume "?LHS"
-  thus "?RHS" by cases
+  assume "?LHS" thus "?RHS" by cases
 next
-  assume "?RHS"
-  thus "?LHS" using big_step.Assign by blast
+  assume "?RHS" thus "?LHS"
+    using big_step.Assign by blast
 qed
 
 lemma inter_seq:
-  "(c1 ;; c2,s1) \<Rightarrow> s3
+    "(c1 ;; c2,s1) \<Rightarrow> s3
     \<longleftrightarrow> (\<exists>s2. ((c1,s1) \<Rightarrow> s2 \<and> (c2,s2) \<Rightarrow> s3))"
   (is "?LHS \<longleftrightarrow> ?RHS")
 proof
-  assume "?LHS"
-  thus "?RHS"
+  assume "?LHS" thus "?RHS"
   proof cases
     case Seq thus ?thesis by auto
   qed
 next
-  assume "?RHS"
-  thus "?LHS" using Seq by blast
+  assume "?RHS" thus "?LHS" using Seq by blast
 qed
 
 lemma while_split:
-  "(WHILE b DO c,s) \<Rightarrow> t
-    \<longleftrightarrow> (
-      \<not> bval b s \<and> t = s
-      \<or> bval b s
-        \<and> (\<exists>s'. (c,s) \<Rightarrow> s'
-            \<and> (WHILE b DO c,s') \<Rightarrow> t))"
+    "(WHILE b DO c,s) \<Rightarrow> t
+    \<longleftrightarrow> ((\<not> bval b s \<and> t = s)
+         \<or> (bval b s
+            \<and> (\<exists>s'.
+                (c,s) \<Rightarrow> s'
+                \<and> (WHILE b DO c,s') \<Rightarrow> t)))"
   (is "?LHS \<longleftrightarrow> ?RHS")
 proof
   assume "?LHS"
   thus "?RHS"
   proof cases
-    case WhileFalse
-    thus ?thesis by auto
+    case WhileFalse thus ?thesis by auto
   next
-    case WhileTrue
-    thus ?thesis by auto
+    case WhileTrue thus ?thesis by auto
   qed
 next
-  assume "?RHS"
-  thus "?LHS"
+  assume "?RHS" thus "?LHS"
     using WhileFalse WhileTrue by blast
 qed
 
 (* Associativity of Seq from 7.2.3 *)
 lemma seq_assoc:
-  "((c1 ;; c2) ;; c3,s) \<Rightarrow> s'
-   \<longleftrightarrow> (c1 ;; (c2 ;; c3),s) \<Rightarrow> s'"
+    "((c1 ;; c2) ;; c3,s) \<Rightarrow> s'
+    \<longleftrightarrow> (c1 ;; (c2 ;; c3),s) \<Rightarrow> s'"
   (is "?LHS \<longleftrightarrow> ?RHS")
 proof
   assume "?LHS"
   then obtain s1 s2 where
-    "(c1,s) \<Rightarrow> s1" and
-    "(c2,s1) \<Rightarrow> s2" and
-    "(c3,s2) \<Rightarrow> s'"
+      "(c1,s) \<Rightarrow> s1" and
+      "(c2,s1) \<Rightarrow> s2" and
+      "(c3,s2) \<Rightarrow> s'"
     using inter_seq by blast
   thus "?RHS" by (simp add: Seq)
 next
   assume "?RHS"
   then obtain s1 s2 where
-    "(c1,s) \<Rightarrow> s1" and
-    "(c2,s1) \<Rightarrow> s2" and
-    "(c3,s2) \<Rightarrow> s'"
+      "(c1,s) \<Rightarrow> s1" and
+      "(c2,s1) \<Rightarrow> s2" and
+      "(c3,s2) \<Rightarrow> s'"
     using inter_seq by blast
-  thus "?LHS"
-    using Seq by blast
+  thus "?LHS" using Seq by blast
 qed
 
 (* Big-step equivalence from 7.2.4 *)
 abbreviation equiv_c :: "com \<Rightarrow> com \<Rightarrow> bool"
   (infix "\<sim>" 50) where
-"c \<sim> c' \<equiv> (\<forall>s. \<forall>t. ((c,s) \<Rightarrow> t = (c',s) \<Rightarrow> t))"
+    "c \<sim> c' \<equiv> (\<forall>s. \<forall>t. ((c,s) \<Rightarrow> t = (c',s) \<Rightarrow> t))"
+
+lemma non_equiv_c:
+    "(\<exists>s. \<exists>t. ((c1,s) \<Rightarrow> t \<and> \<not>((c2,s) \<Rightarrow> t)))
+    \<Longrightarrow> \<not>(c1 \<sim> c2)"
+proof -
+  assume "\<exists>s. \<exists>t. ((c1,s) \<Rightarrow> t \<and> \<not>((c2,s) \<Rightarrow> t))"
+  hence "\<exists>s. \<exists>t. \<not>((c1,s) \<Rightarrow> t \<longrightarrow> (c2,s) \<Rightarrow> t)" by simp
+  hence "\<exists>s. \<exists>t. ((c1,s) \<Rightarrow> t \<noteq> (c2,s) \<Rightarrow> t)" by auto
+  hence "\<not>(\<forall>s. \<forall>t. ((c1,s) \<Rightarrow> t = (c2,s) \<Rightarrow> t))" by simp
+  thus ?thesis by simp
+qed
+
 
 (* While is equivalent to a single unfold of itself *)
 lemma while_is_unfolded_while:
-  "(WHILE b DO c)
+    "(WHILE b DO c)
     \<sim> (IF b THEN c ;; WHILE b DO c ELSE SKIP)"
   (is "?LHS \<sim> ?RHS")
 proof -
   have "(?RHS,s) \<Rightarrow> t" if assm: "(?LHS,s) \<Rightarrow> t" for s t
   proof -
-    from assm show ?thesis
+    show ?thesis using assm
     proof cases
       case WhileTrue
-      from this `bval b s` `(?LHS,s) \<Rightarrow> t`
-      obtain s'
-        where "(c,s) \<Rightarrow> s'" and "(?LHS,s') \<Rightarrow> t"
-        by blast
+      then obtain s' where
+          "(c,s) \<Rightarrow> s'" and
+          "(?LHS,s') \<Rightarrow> t"
+        using `bval b s` `(?LHS,s) \<Rightarrow> t` by blast
       hence "(c ;; ?LHS,s) \<Rightarrow> t" by (rule Seq)
       thus ?thesis using `bval b s` by auto
     next
-      case WhileFalse
-      thus ?thesis by auto
+      case WhileFalse thus ?thesis by auto
     qed
   qed
   moreover
@@ -223,9 +256,10 @@ proof -
     from assm show ?thesis
     proof cases
       case IfTrue
-      from this inter_seq obtain s'
-        where "(c,s) \<Rightarrow> s'" and "(?LHS,s') \<Rightarrow> t"
-        by blast
+      then obtain s' where
+          "(c,s) \<Rightarrow> s'" and
+          "(?LHS,s') \<Rightarrow> t"
+        using inter_seq by blast
       thus ?thesis using IfTrue by blast
     next
       case IfFalse
@@ -240,64 +274,1769 @@ qed
 (* The previous proof is likely clearer,
    but all that inductive_case stuff allows
    full auto here *)
-lemma "(WHILE b DO c) \<sim> (IF b THEN c ;; WHILE b DO c ELSE SKIP)"
+lemma
+    "(WHILE b DO c)
+    \<sim> (IF b THEN (c ;; WHILE b DO c) ELSE SKIP)"
   by blast
 
 (* A command in both if clauses is equivalent
    to the command (from 7.2.4) *)
 lemma if_both_com_is_com:
-  "(IF b THEN c ELSE c) \<sim> c"
+    "(IF b THEN c ELSE c) \<sim> c"
   by blast
 
 (* Equivalent commands yeild equivalent while loops
    (from 7.2.4) *)
 lemma while_equiv_complex:
-  "\<lbrakk> (WHILE b DO c,s) \<Rightarrow> t ; c \<sim> c' \<rbrakk>
+    "\<lbrakk> (WHILE b DO c,s) \<Rightarrow> t ; c \<sim> c' \<rbrakk>
     \<Longrightarrow> (WHILE b DO c',s) \<Rightarrow> t"
-  apply (induction "WHILE b DO c" s t arbitrary: b c rule: big_step_induct)
-   apply blast
-  apply blast
+  apply (
+      induction "WHILE b DO c" s t
+      arbitrary: b c
+      rule: big_step_induct)
+  apply blast+
   done
 
 corollary while_equiv:
-  "c \<sim> c' \<Longrightarrow> ((WHILE b DO c) \<sim> (WHILE b DO c'))"
+    "c \<sim> c' \<Longrightarrow> ((WHILE b DO c) \<sim> (WHILE b DO c'))"
   by (meson while_equiv_complex)
+
+lemma if_guard_equiv:
+    "bval b1 s = bval b2 s
+    \<Longrightarrow> (IF b1 THEN c1 ELSE c2,s) \<Rightarrow> t
+        = (IF b2 THEN c1 ELSE c2,s) \<Rightarrow> t"
+  by auto
+
 
 (* Big-step equivalence is an equivalence relation *)
 theorem refl_equiv_c: "c \<sim> c" by auto
 theorem sym_equiv_c: "c1 \<sim> c2 \<Longrightarrow> c2 \<sim> c1" by auto
-theorem trans_equiv_c: "c1 \<sim> c2 \<and> c2 \<sim> c3 \<Longrightarrow> c1 \<sim> c3"
+theorem trans_equiv_c:
+    "c1 \<sim> c2 \<and> c2 \<sim> c3 \<Longrightarrow> c1 \<sim> c3"
   by auto
+
 
 (* IMP is deterministic from 7.2.5 *)
 theorem imp_deterministic:
-  "(c,s) \<Rightarrow> t \<Longrightarrow> (c,s) \<Rightarrow> t' \<Longrightarrow> t' = t"
+    "(c,s) \<Rightarrow> t \<Longrightarrow> (c,s) \<Rightarrow> t' \<Longrightarrow> t' = t"
 proof (induction arbitrary: t' rule: big_step.induct)
   fix b c s s1 t t'
-  assume "bval b s"
-    and "(c,s) \<Rightarrow> s1"
-    and "(WHILE b DO c,s1) \<Rightarrow> t"
-  assume IHc: "\<And>t'. (c,s) \<Rightarrow> t' \<Longrightarrow> t' = s1"
-  assume IHw: "\<And>t'. (WHILE b DO c,s1) \<Rightarrow> t' \<Longrightarrow> t' = t"
-  assume "(WHILE b DO c,s) \<Rightarrow> t'"
-  with `bval b s` obtain s1' where
-    c: "(c,s) \<Rightarrow> s1'" and
-    w: "(WHILE b DO c,s1') \<Rightarrow> t'"
-    by auto
-  from c IHc have "s1' = s1" by blast
-  with w IHw show "t' = t" by blast
+  assume
+      "bval b s" and
+      IHc: "\<And>t'. (c,s) \<Rightarrow> t' \<Longrightarrow> t' = s1" and
+      IHw: "\<And>t'. (WHILE b DO c,s1) \<Rightarrow> t' \<Longrightarrow> t' = t" and
+      "(WHILE b DO c,s) \<Rightarrow> t'"
+  then obtain s1' where
+      c: "(c,s) \<Rightarrow> s1'" and
+      w: "(WHILE b DO c,s1') \<Rightarrow> t'"
+    using WhileE by metis
+  hence "s1' = s1" using IHc by blast
+  thus "t' = t" using w IHw by blast
 qed blast+
+
+corollary diff_end_impl_diff_com:
+    "\<lbrakk> t \<noteq> t'; (c,s) \<Rightarrow> t; (c',s) \<Rightarrow> t' \<rbrakk>
+    \<Longrightarrow> \<not>(c \<sim> c')"
+  using imp_deterministic by force
+
+(* Small-step determinism *)
+theorem small_step_imp_deterministic:
+    "cs \<rightarrow> cs1 \<Longrightarrow> cs \<rightarrow> cs2 \<Longrightarrow> cs2 = cs1"
+  by (induction arbitrary: cs2 rule: small_step.induct,
+      blast+)
+
 
 (* Reflexive transitive closure from 4.5.2 *)
 (* Needed for closure of small-step semantic *)
-inductive star :: "('a \<Rightarrow> 'a \<Rightarrow> bool) \<Rightarrow> 'a \<Rightarrow> 'a \<Rightarrow> bool"
+inductive star ::
+    "('a \<Rightarrow> 'a \<Rightarrow> bool) \<Rightarrow> 'a \<Rightarrow> 'a \<Rightarrow> bool"
   for r where
-refl: "star r x x" |
-step: "r x y \<Longrightarrow> star r y z \<Longrightarrow> star r x z"
+    refl: "star r x x" |
+    step: "r x y \<Longrightarrow> star r y z \<Longrightarrow> star r x z"
+
+lemma star_trans:
+    "star r x y \<Longrightarrow> star r y z \<Longrightarrow> star r x z"
+proof (induction rule: star.induct)
+  case refl thus ?case by simp
+next
+  case step thus ?case by (metis star.step)
+qed
+
+lemmas star_induct =
+    star.induct[
+        of "r :: 'a * 'b \<Rightarrow> 'a * 'b \<Rightarrow> bool",
+        split_format(complete)]
+declare star.refl[simp,intro]
+lemma star_base[simp,intro]: "r x y \<Longrightarrow> star r x y"
+  by (meson star.simps)
+
+inductive star2 ::
+    "('a \<Rightarrow> 'a \<Rightarrow> bool) \<Rightarrow> 'a \<Rightarrow> 'a \<Rightarrow> bool"
+  for r where
+    refl2: "star2 r x x" |
+    step2: "star2 r x y \<Longrightarrow> r y z \<Longrightarrow> star2 r x z"
+
+lemma star2_impl_star: "star2 r x y \<Longrightarrow> star r x y"
+proof (induction rule: star2.induct)
+  case refl2 thus ?case by simp
+next
+  case step2 thus ?case by (meson star_base star_trans)
+qed
+
+lemma rel_impl_star2: "r x y \<Longrightarrow> star2 r x y"
+  by (meson star2.refl2 star2.step2)
+
+lemma star2_transpose:
+    "star2 r y z \<Longrightarrow> r x y \<Longrightarrow> star2 r x z"
+proof (induction rule: star2.induct)
+  case refl2 thus ?case by (rule rel_impl_star2)
+next
+  case step2 thus ?case by (meson star2.step2)
+qed
+
+lemma star_impl_star2: "star r x y \<Longrightarrow> star2 r x y"
+proof (induction rule: star.induct)
+  case refl thus ?case by (rule star2.refl2)
+next
+  case step thus ?case by (simp add: star2_transpose)
+qed
+
+lemmas star2_induct =
+    star2.induct[
+        of "r :: 'a * 'b \<Rightarrow> 'a * 'b \<Rightarrow> bool",
+        split_format(complete)]
 
 (* Closure of small-step sequences from 7.3 *)
-abbreviation small_step_closure :: "com \<times> state \<Rightarrow> com \<times> state \<Rightarrow> bool"
+abbreviation small_step_closure ::
+    "com \<times> state \<Rightarrow> com \<times> state \<Rightarrow> bool"
   (infix "\<rightarrow>*" 55) where
-"x \<rightarrow>* y \<equiv> star small_step x y"
+    "x \<rightarrow>* y \<equiv> star small_step x y"
+
+(* Small-step based determinism proof from 7.3 *)
+lemma imp_deterministic_small_step:
+    "\<lbrakk> cs \<rightarrow> cs'; cs \<rightarrow> cs'' \<rbrakk> \<Longrightarrow> cs'' = cs'"
+  by (induction
+        arbitrary: cs''
+        rule: small_step.induct,
+      blast+)
+
+(* Small-step equivalence is preserved through the
+   addition of a sequential suffix, proof from 7.3 *)
+lemma seq_suffix:
+    "(c1, s1) \<rightarrow>* (c, s2)
+    \<Longrightarrow> (c1 ;; c2, s1) \<rightarrow>* (c ;; c2, s2)"
+proof (induction rule: star_induct)
+  case refl thus ?case by simp
+next
+  case step thus ?case by (meson Seq2 star.simps)
+qed
+
+(* Sequential transitivity of small steps *)
+lemma star_seq:
+    "\<lbrakk> (c1, s1) \<rightarrow>* (SKIP, s2); (c2, s2) \<rightarrow>* (SKIP, s3) \<rbrakk>
+    \<Longrightarrow> (c1 ;; c2, s1) \<rightarrow>* (SKIP, s3)"
+  by (blast intro: star.step seq_suffix star_trans)
+
+(* Big-step implies small-step eventual termination,
+   from 7.3.1 *)
+theorem big_step_impl_small_term:
+    "cs \<Rightarrow> t \<Longrightarrow> cs \<rightarrow>* (SKIP,t)"
+proof (induction rule: big_step.induct)
+  fix s
+  show "(SKIP, s) \<rightarrow>* (SKIP, s)"
+    by (rule star.intros(1))
+next
+  fix x a s
+  show "(x ::= a, s) \<rightarrow>* (SKIP, s(x := aval a s))"
+    using star.simps small_step.Assign by metis
+next
+  fix c1 s1 s2 c2 s3
+  assume
+      "(c1, s1) \<rightarrow>* (SKIP, s2)"
+      and "(c2, s2) \<rightarrow>* (SKIP, s3)"
+  thus "(c1 ;; c2, s1) \<rightarrow>* (SKIP, s3)"
+    by (rule star_seq)
+next
+  fix b s c1 t c2
+  assume "bval b s" and "(c1,s) \<Rightarrow> t"
+  hence "(IF b THEN c1 ELSE c2,s) \<Rightarrow> t"
+    by (rule big_step.IfTrue)
+  assume "(c1,s) \<rightarrow>* (SKIP,t)"
+  thus "(IF b THEN c1 ELSE c2,s) \<rightarrow>* (SKIP,t)"
+    using `bval b s` small_step.IfTrue
+    by (meson star.simps)
+next
+  fix b s c1 t c2
+  assume "\<not>bval b s" and "(c2,s) \<Rightarrow> t"
+  hence "(IF b THEN c1 ELSE c2,s) \<Rightarrow> t"
+    by (rule big_step.IfFalse)
+  assume "(c2,s) \<rightarrow>* (SKIP,t)"
+  thus "(IF b THEN c1 ELSE c2,s) \<rightarrow>* (SKIP,t)"
+    using `\<not>bval b s` small_step.IfFalse
+    by (meson star.simps)
+next
+  fix b s c
+  have
+      while_unfold: "(WHILE b DO c,s)
+      \<rightarrow> (IF b THEN (c ;; WHILE b DO c) ELSE SKIP,s)"
+    by blast
+  assume "\<not>bval b s"
+  hence
+      "(IF b THEN (c ;; WHILE b DO c) ELSE SKIP,s)
+      \<rightarrow> (SKIP,s)"
+    by (rule small_step.IfFalse)
+  thus "(WHILE b DO c,s) \<rightarrow>* (SKIP,s)"
+    using while_unfold by (metis star.simps)
+next
+  fix b s c s' t
+  have
+      while_unfold: "(WHILE b DO c,s)
+      \<rightarrow> (IF b THEN (c ;; WHILE b DO c) ELSE SKIP,s)"
+    by blast
+  assume "bval b s"
+  hence
+      while_unroll: "(
+          IF b
+          THEN (c ;; WHILE b DO c)
+          ELSE SKIP,s)
+      \<rightarrow> (c ;; WHILE b DO c,s)"
+    by simp
+  assume
+      "(WHILE b DO c,s') \<rightarrow>* (SKIP,t)"
+      and "(c,s) \<rightarrow>* (SKIP,s')"
+  hence "(c ;; WHILE b DO c,s) \<rightarrow>* (SKIP,t)"
+    by (simp add: star_seq)
+  thus "(WHILE b DO c,s) \<rightarrow>* (SKIP,t)"
+    using while_unfold while_unroll by (meson star.step)
+qed
+
+(* Small-step prepends to big-step, from 7.3 *)
+lemma small_step_prepend_big_step:
+    "\<lbrakk> cs \<rightarrow> cs'; cs' \<Rightarrow> t \<rbrakk> \<Longrightarrow> cs \<Rightarrow> t"
+  by (induction arbitrary: t rule: small_step.induct,
+      auto)
+
+(* Small-step eventual termination implies big-step,
+   from 7.3 *)
+theorem small_term_impl_big_step:
+    "cs \<rightarrow>* (SKIP,t) \<Longrightarrow> cs \<Rightarrow> t"
+proof (induction cs "(SKIP,t)" rule: star.induct)
+  case refl thus ?case by (rule big_step.Skip)
+next
+  case step thus ?case
+    by (simp add: small_step_prepend_big_step)
+qed
+
+corollary big_step_small_term_equiv:
+    "cs \<Rightarrow> t \<longleftrightarrow> cs \<rightarrow>* (SKIP,t)"
+  using
+      big_step_impl_small_term
+      small_term_impl_big_step
+  by blast
+
+definition final :: "(com \<times> state) \<Rightarrow> bool" where
+    "final cs \<longleftrightarrow> \<not>(\<exists>cs'. cs \<rightarrow> cs')"
+
+corollary final_split:
+    "final (c,s) \<longleftrightarrow> \<not>(\<exists>d. \<exists>t. (c,s) \<rightarrow> (d,t))"
+  by (simp add: final_def)
+
+(* Only SKIP is in final state, from 7.3 *)
+lemma skip_finality: "final (c,s) \<longleftrightarrow> (c = SKIP)"
+  by (simp add: final_def, induction c, blast+)
+
+theorem big_step_term:
+    "(\<exists>t. cs \<Rightarrow> t) \<longleftrightarrow> (\<exists>cs'. (cs \<rightarrow>* cs' \<and> final cs'))"
+  by (simp add: big_step_small_term_equiv skip_finality)
+
+theorem small_step_tail_equiv:
+    "(c1 \<sim> c2)
+    \<longleftrightarrow> (\<forall>s.\<forall>t. (c1,s) \<rightarrow>* (SKIP,t)
+        = (c2,s) \<rightarrow>* (SKIP,t))"
+    using
+      big_step_impl_small_term
+      small_term_impl_big_step
+    by blast
+
+lemma small_step_antireflexivity:
+    "((c,s) \<rightarrow> (d,t)) \<Longrightarrow> (d \<noteq> c)"
+  by (induction rule: small_step_induct, simp_all)
+
+lemma non_final_successor:
+    "(\<not> final (c,s))
+    \<longleftrightarrow> (\<exists>d. \<exists>t. (c,s) \<rightarrow>* (d,t) \<and> (d \<noteq> c))"
+proof
+  assume "\<not> final (c,s)"
+  hence "\<exists>d. \<exists>t. (c,s) \<rightarrow> (d,t)"
+    by (simp add: final_def)
+  hence "\<exists>d. \<exists>t. (c,s) \<rightarrow> (d,t) \<and> (d \<noteq> c)"
+    using small_step_antireflexivity
+    by blast
+  have "((c,s) \<rightarrow> (d,t)) \<Longrightarrow> ((c,s) \<rightarrow>* (d,t))" for d t
+    by simp
+  hence "\<exists>d. \<exists>t. (c,s) \<rightarrow>* (d,t)"
+    using `\<exists>d. \<exists>t. (c,s) \<rightarrow> (d,t)`
+    by auto
+  thus "\<exists>d. \<exists>t. (c,s) \<rightarrow>* (d,t) \<and> (d \<noteq> c)"
+    using `\<exists>d t. (c, s) \<rightarrow> (d, t) \<and> d \<noteq> c`
+    by blast
+next
+  assume "\<exists>d. \<exists>t. (c,s) \<rightarrow>* (d,t) \<and> (d \<noteq> c)"
+  hence "\<exists>d. \<exists>t. (c,s) \<rightarrow> (d,t)"
+    using prod.inject small_step.cases star.simps
+    by (smt (verit))
+  hence "\<not> (\<not> (\<exists>d. \<exists>t. (c,s) \<rightarrow> (d,t)))" by simp
+  thus "\<not> final (c,s)"
+    using final_split by blast
+qed
+
+thm impI[of "foo" "bar"]
+thm impI[of "(c,s) \<noteq> (d,t)" "(\<exists>c'. \<exists>s'. (c,s) \<rightarrow> (c',s') \<and> (c',s') \<rightarrow>* (d,t))"]
+thm iffI[of b c]
+
+theorem big_step_equiv_is_small_term_equiv:
+    "(\<forall>s. \<forall>t. ((a,s) \<rightarrow>* (SKIP,t) = (b,s) \<rightarrow>* (SKIP,t)))
+    \<longleftrightarrow> (a \<sim> b)"
+  by (simp add: big_step_small_term_equiv)
+
+lemma penult_star_state:
+    "((c \<noteq> d \<or> s \<noteq> t) \<and> (c,s) \<rightarrow>* (d,t))
+    \<Longrightarrow> \<exists>d'. \<exists>t'. ((c,s) \<rightarrow>* (d',t')
+                  \<and> (d',t') \<rightarrow> (d,t))"
+proof -
+  assume "(c \<noteq> d \<or> s \<noteq> t) \<and> (c,s) \<rightarrow>* (d,t)"
+  hence "\<exists>c'. \<exists>s'. (c,s) \<rightarrow> (c',s') \<and> (c',s') \<rightarrow>* (d,t)"
+    using
+      SmallSkipE
+      final_split
+      imp_deterministic_small_step
+      prod.inject
+      skip_finality
+      star.simps
+    by (smt (verit, del_insts))
+  then obtain c' s' where
+      "(c,s) \<rightarrow> (c',s') \<and> (c',s') \<rightarrow>* (d,t)"
+    by auto
+  hence "(c',s') \<rightarrow>* (d,t)" by simp
+  hence "star2 small_step (c',s') (d,t)"
+    by (rule star_impl_star2)
+  thus "\<exists>d'. \<exists>t'. (c,s) \<rightarrow>* (d',t') \<and> (d',t') \<rightarrow> (d,t)"
+  proof (induction "(c',s')" "(d,t)" rule: star2.induct)
+    case refl2
+    hence "(c',s') = (d,t)" by simp
+    hence "(c,s) \<rightarrow>* (c,s) \<and> (c,s) \<rightarrow> (d,t)"
+      using `(c, s) \<rightarrow> (c', s') \<and> (c', s') \<rightarrow>* (d, t)`
+      by blast
+    thus
+        "\<exists>d'. \<exists>t'. (c,s) \<rightarrow>* (d',t')
+                   \<and> (d',t') \<rightarrow> (d,t)"
+      by auto
+  next
+    case (step2 a)
+    hence "(c',s') \<rightarrow>* a"
+      by (simp add: star2_impl_star)
+    hence "(c,s) \<rightarrow>* a"
+      using
+        `(c,s) \<rightarrow> (c',s')
+        \<and> (c',s') \<rightarrow>* (d,t)`
+      by (meson star.step)
+    have "a \<rightarrow> (d,t)"
+      by (rule local.step2(3))
+    have "\<exists>d'. \<exists>t'. a = (d',t')"
+      by (rule Product_Type.surj_pair)
+    thus
+        "\<exists>d'. \<exists>t'. (c,s) \<rightarrow>* (d',t')
+                   \<and> (d',t') \<rightarrow> (d,t)"
+      using `(c,s) \<rightarrow>* a` step2.hyps(3)
+      by blast
+  qed
+qed
+
+inductive small_step_count ::
+    "com \<times> state \<Rightarrow> com \<times> state \<Rightarrow> nat \<Rightarrow> bool"
+  where
+Self: "small_step_count (c,s) (c,s) 0" |
+Step:
+    "(c,s) \<rightarrow> (d,t)
+    \<Longrightarrow> small_step_count (c,s) (d,t) 1" |
+Following:
+    "n1 + n2 > 1
+    \<Longrightarrow> small_step_count (c1,s1) (c2,s2) n1
+    \<Longrightarrow> small_step_count (c2,s2) (c3,s3) n2
+    \<Longrightarrow> small_step_count (c1,s1) (c3,s3) (n1 + n2)"
+
+theorem zero_count_same:
+    "small_step_count (c,s) (d,t) 0 \<longleftrightarrow> (c,s) = (d,t)"
+proof
+  assume "small_step_count (c,s) (d,t) 0"
+  thus "(c,s) = (d,t)"
+  proof cases
+    case Self
+    thus "(c,s) = (d,t)"
+      by simp
+  next
+    case Step
+    hence "0 = 1 \<Longrightarrow> (c,s) = (d,t)"
+      by simp
+    thus ?thesis
+      using local.Step(1)
+      by blast
+  next
+    case (Following n1 n2 c2 s2)
+    hence "0 = n1 + n2 \<and> 0 < n1 + n2"
+      by simp
+    thus ?thesis
+      by auto
+  qed
+next
+  assume "(c,s) = (d,t)"
+  thus "small_step_count (c,s) (d,t) 0"
+    using small_step_count.Self
+    by auto
+qed
+
+lemma leads_to_count:
+    "(c,s) \<rightarrow>* (d,t)
+    \<Longrightarrow> \<exists>n. small_step_count (c,s) (d,t) n"
+proof (induction c s d t rule: star_induct)
+  case refl
+  thus ?case
+    using small_step_count.Self
+    by blast
+next
+  case (step c s c' s' d t)
+  hence
+      "(c,s) \<rightarrow> (c',s')"
+      "(c',s') \<rightarrow>* (d,t)"
+      "\<exists>n. small_step_count (c',s') (d,t) n"
+    by auto
+  hence "small_step_count (c,s) (c',s') 1"
+    using small_step_count.Step
+    by simp
+  have "(c',s') = (d,t) \<or> (c',s') \<noteq> (d,t)"
+    by simp
+  thus "\<exists>n. small_step_count (c,s) (d,t) n"
+  proof (elim disjE)
+    assume "(c',s') = (d,t)"
+    hence "small_step_count (c,s) (d,t) 1"
+      using `small_step_count (c,s) (c',s') 1`
+      by blast
+    thus "\<exists>n. small_step_count (c,s) (d,t) n"
+      by (rule HOL.exI)
+  next
+    assume "(c',s') \<noteq> (d,t)"
+    then obtain n' where
+        "small_step_count (c',s') (d,t) n'"
+      using `\<exists>n. small_step_count (c',s') (d,t) n`
+      by blast
+    hence "n' \<noteq> 0"
+      using
+        `(c',s') \<noteq> (d,t)`
+        zero_count_same
+      by force
+    hence "1 + n' > 1"
+      by simp
+    hence "small_step_count (c,s) (d,t) (1+n')"
+      using
+        small_step_count.Following
+        `small_step_count (c,s) (c',s') 1`
+        `small_step_count (c',s') (d,t) n'`
+      by blast
+    thus "\<exists>n. small_step_count (c,s) (d,t) n"
+      by (rule HOL.exI)
+  qed
+qed
+
+theorem count_leads_to:
+    "(\<exists>n. small_step_count (c,s) (d,t) n)
+    \<longleftrightarrow> ((c,s) \<rightarrow>* (d,t))"
+proof
+  assume "\<exists>n. small_step_count (c,s) (d,t) n"
+  then obtain n' where
+      "small_step_count (c,s) (d,t) n'"
+    by auto
+  thus "(c,s) \<rightarrow>* (d,t)"
+  proof induction
+    case (Self c s)
+    thus "(c,s) \<rightarrow>* (c,s)"
+      by simp
+  next
+    case (Step c s d t)
+    hence "(c,s) \<rightarrow> (d,t)"
+      by simp
+    thus "(c,s) \<rightarrow>* (d,t)"
+      by simp
+  next
+    case (Following n1 n2 c1 s1 c2 s2 c3 s3)
+    hence
+        "small_step_count (c1,s1) (c2,s2) n1
+        \<and> small_step_count (c2,s2) (c3,s3) n2"
+        "(c1,s1) \<rightarrow>* (c2,s2) \<and> (c2,s2) \<rightarrow>* (c3,s3)"
+      by auto
+    hence "small_step_count (c1,s1) (c3,s3) (n1+n2)"
+      using
+        local.Following.hyps(1)
+        small_step_count.Following
+      by auto
+    have "(c1,s1) \<rightarrow>* (c3,s3)"
+      using
+        `(c1,s1) \<rightarrow>* (c2,s2) \<and> (c2,s2) \<rightarrow>* (c3,s3)`
+        star_trans
+      by meson
+    thus ?case
+      by simp
+  qed
+next
+  assume "(c,s) \<rightarrow>* (d,t)"
+  thus "\<exists>n. small_step_count (c,s) (d,t) n"
+    by (simp add: leads_to_count)
+qed
+
+theorem one_count_is_step:
+    "small_step_count (c,s) (d,t) 1 \<longleftrightarrow> (c,s) \<rightarrow> (d,t)"
+proof
+  assume "small_step_count (c,s) (d,t) 1"
+  thus "(c,s) \<rightarrow> (d,t)"
+  proof cases
+    case Self
+    hence "1 = 0"
+      by simp
+    thus "(c,s) \<rightarrow> (d,t)"
+      using local.Self(3)
+      by simp
+  next
+    case Step
+    thus "(c,s) \<rightarrow> (d,t)"
+      by simp
+  next
+    case (Following n1 n2 c2 s2)
+    hence "1 = n1 + n2 \<and> 1 < n1 + n2"
+      by simp
+    thus "(c,s) \<rightarrow> (d,t)"
+      using local.Following
+      by linarith
+  qed
+next
+  assume "(c,s) \<rightarrow> (d,t)"
+  thus "small_step_count (c,s) (d,t) 1"
+    by (rule small_step_count.Step)
+qed
+
+lemma count_penult_step_lt:
+    "(small_step_count (c,s) (d,t) n \<and> n > 1)
+    \<Longrightarrow> (\<exists>d'. \<exists>t'. small_step_count (c,s) (d',t') (n-1)
+        \<and> small_step_count (d',t') (d,t) 1)"
+proof -
+  assume "small_step_count (c,s) (d,t) n \<and> n > 1"
+  hence
+      "small_step_count (c,s) (d,t) n"
+      "n > 1"
+    by auto
+  thus
+      "\<exists>d'. \<exists>t'. small_step_count (c,s) (d',t') (n-1)
+      \<and> small_step_count (d',t') (d,t) 1"
+  proof (induction rule: small_step_count.induct)
+    case (Self c s)
+    hence "1 < 0" by simp
+    thus ?case by auto
+  next
+    case (Step c s d t)
+    hence "1 < 1" by simp
+    thus ?case by auto
+  next
+    case (Following n1 n2 c s d2 t2 d t)
+    hence "n2 > 1 \<or> n2 = 1 \<or> (n2 = 0 \<and> n1 > 1)"
+      by auto
+    thus ?case
+    proof (elim disjE)
+      assume "n2 > 1"
+      hence
+          "\<exists>d'. \<exists>t'.
+          small_step_count (d2,t2) (d',t') (n2-1)
+          \<and> small_step_count (d',t') (d,t) 1"
+        by (rule local.Following(5))
+      then obtain d' t' where
+          "small_step_count (d2,t2) (d',t') (n2-1)
+          \<and> small_step_count (d',t') (d,t) 1"
+        by auto
+      hence
+          "small_step_count (d2,t2) (d',t') (n2-1)"
+          "small_step_count (d',t') (d,t) 1"
+        by auto
+      have "n1 = 0 \<or> n1 + n2 > 2"
+        using `1 < n2`
+        by linarith
+      hence "small_step_count (c,s) (d',t') (n1+n2-1)"
+        using
+          Following.hyps(2)
+          `1 < n2`
+          `small_step_count (d2,t2) (d',t') (n2-1)`
+          small_step_count.Following
+          zero_count_same
+        by (smt (verit, best)
+            Nat.add_diff_assoc
+            add_cancel_left_left
+            less_diff_conv
+            less_imp_le
+            one_add_one)
+      thus
+          "\<exists>d'. \<exists>t'.
+          small_step_count (c,s) (d',t') (n1+n2-1)
+          \<and> small_step_count (d',t') (d,t) 1"
+        using `small_step_count (d',t') (d,t) 1`
+        by blast
+    next
+      assume "n2 = 1"
+      hence "small_step_count (d2,t2) (d,t) 1"
+        using local.Following.hyps(3)
+        by blast
+      have "n1 + n2 - 1 = n1"
+        using `n2 = 1`
+        by simp
+      hence
+          "small_step_count (c,s) (d2,t2) (n1+n2-1)
+          \<and> small_step_count (d2,t2) (d,t) 1"
+        using
+          local.Following.hyps(2)
+          `small_step_count (d2,t2) (d,t) 1`
+        by presburger
+      thus
+          "\<exists>d'. \<exists>t'.
+          small_step_count (c,s) (d',t') (n1+n2-1)
+          \<and> small_step_count (d',t') (d,t) 1"
+        by auto
+    next
+      assume "n2 = 0 \<and> n1 > 1"
+      hence
+          "n2 = 0"
+          "n1 > 1"
+        by auto
+      hence "small_step_count (d2,t2) (d,t) 0"
+        using local.Following.hyps(3)
+        by blast
+      hence "(d,t) = (d2,t2)"
+        using zero_count_same
+        by simp
+      have "n1 + n2 - 1 = n1 - 1"
+        using
+          `n2 = 0`
+          `n1 > 1`
+        by simp
+      have
+          "\<exists>d'. \<exists>t'.
+          small_step_count (c,s) (d',t') (n1-1)
+          \<and> small_step_count (d',t') (d,t) 1"
+        using
+          Following.IH(1)
+          `1 < n1`
+          `(d,t) = (d2,t2)`
+        by simp
+      thus
+          "\<exists>d'. \<exists>t'.
+          small_step_count (c,s) (d',t') (n1+n2-1)
+          \<and> small_step_count (d',t') (d,t) 1"
+        using
+          `(d,t) = (d2,t2)`
+          `n1 + n2 - 1 = n1 - 1`
+        by simp
+    qed
+  qed
+qed
+
+corollary count_penult_step:
+    "(small_step_count (c,s) (d,t) n \<and> n \<ge> 1)
+    \<Longrightarrow> (\<exists>d'. \<exists>t'. small_step_count (c,s) (d',t') (n-1)
+        \<and> small_step_count (d',t') (d,t) 1)"
+proof -
+  assume "small_step_count (c,s) (d,t) n \<and> 1 \<le> n"
+  hence "n = 1 \<or> n > 1"
+    by auto
+  thus
+      "\<exists>d'. \<exists>t'.
+      small_step_count (c,s) (d',t') (n-1)
+      \<and> small_step_count (d',t') (d,t) 1"
+  proof (elim disjE)
+    assume "n = 1"
+    have "small_step_count (c,s) (c,s) 0"
+      by (rule small_step_count.Self)
+    hence "small_step_count (c,s) (c,s) (n-1)"
+      using `n = 1`
+      by simp
+    have "small_step_count (c,s) (d,t) n"
+      using `small_step_count (c,s) (d,t) n \<and> 1 \<le> n`
+      by simp
+    hence "small_step_count (c,s) (d,t) 1"
+      using `n = 1`
+      by simp
+    thus
+        "\<exists>d'. \<exists>t'. small_step_count (c,s) (d',t') (n-1)
+        \<and> small_step_count (d',t') (d,t) 1"
+      using `small_step_count (c,s) (c,s) (n-1)`
+      by auto
+  next
+    assume "n > 1"
+    have "small_step_count (c,s) (d,t) n"
+      using `small_step_count (c,s) (d,t) n \<and> 1 \<le> n`
+      by simp
+    thus
+        "\<exists>d'. \<exists>t'. small_step_count (c,s) (d',t') (n-1)
+        \<and> small_step_count (d',t') (d,t) 1"
+        using
+          count_penult_step_lt
+          `n > 1`
+      by blast
+  qed
+qed
+
+theorem equiv_count_impl_equiv_state:
+    "(small_step_count (c,s) (d1,t1) n
+      \<and> small_step_count (c,s) (d2,t2) n)
+    \<Longrightarrow> (d1,t1) = (d2,t2)"
+proof (induction n arbitrary: d1 t1 d2 t2)
+  case 0
+  hence
+      "small_step_count (c,s) (d1,t1) 0"
+      "small_step_count (c,s) (d2,t2) 0"
+    by auto
+  hence
+      "(c,s) = (d1,t1)"
+      "(c,s) = (d2,t2)"
+    using zero_count_same
+    by simp_all
+  thus "(d1,t1) = (d2,t2)"
+    by simp
+next
+  case (Suc n)
+  hence
+      "small_step_count (c,s) (d1,t1) (Suc n)"
+      "small_step_count (c,s) (d2,t2) (Suc n)"
+    by auto
+  then obtain d1' t1' where
+      "small_step_count (c,s) (d1',t1') n
+      \<and> small_step_count (d1',t1') (d1,t1) 1"
+    using
+      count_penult_step
+      small_step_count.Self
+    by fastforce
+  obtain d2' t2' where
+      "small_step_count (c,s) (d2',t2') n
+      \<and> small_step_count (d2',t2') (d2,t2) 1"
+    using
+      count_penult_step
+      small_step_count.Self
+      `small_step_count (c,s) (d2,t2) (Suc n)`
+    by fastforce
+  hence
+      "small_step_count (c,s) (d1',t1') n
+      \<and> small_step_count (c,s) (d2',t2') n"
+    using
+      `small_step_count (c,s) (d1',t1') n
+      \<and> small_step_count (d1',t1') (d1,t1) 1`
+    by blast
+  hence "(d1',t1') = (d2',t2')"
+    by (rule local.Suc.IH)
+  hence "small_step_count (d1',t1') (d2,t2) 1"
+    using
+      `small_step_count (c,s) (d2',t2') n
+      \<and> small_step_count (d2',t2') (d2,t2) 1`
+    by blast
+  hence "(d1',t1') \<rightarrow> (d1,t1) \<and> (d1',t1') \<rightarrow> (d2,t2)"
+    using
+      `small_step_count (c,s) (d1',t1') n
+      \<and> small_step_count (d1',t1') (d1,t1) 1`
+      one_count_is_step
+    by blast
+  thus "(d1,t1) = (d2,t2)"
+    using small_step_imp_deterministic
+    by blast
+qed
+
+corollary small_step_count_split:
+    "n1 \<ge> n2 \<and> n2 \<ge> 0
+      \<and> small_step_count (c,s) (d,t) n1
+    \<Longrightarrow> \<exists>c'. \<exists>s'. (
+      small_step_count (c,s) (c',s') (n1-n2)
+      \<and> small_step_count (c',s') (d,t) n2)"
+proof (induction n2)
+  case 0
+  hence "small_step_count (c,s) (d,t) n1"
+    by simp
+  hence "small_step_count (c,s) (d,t) (n1-0)"
+    by simp
+  have "small_step_count (d,t) (d,t) 0"
+    by (rule small_step_count.Self)
+  thus
+      "\<exists>c'. \<exists>s'. small_step_count (c,s) (c',s') (n1-0)
+      \<and> small_step_count (c',s') (d,t) 0"
+    using `small_step_count (c,s) (d,t) (n1-0)`
+    by auto
+next
+  case (Suc n2)
+  hence
+      "(Suc n2) \<le> n1"
+      "0 \<le> (Suc n2)"
+      "small_step_count (c,s) (d,t) n1"
+    by auto
+  hence "n2 < n1"
+    using `(Suc n2) \<le> n1`
+    by simp
+  hence "n2 \<le> n1"
+    by simp
+  have "0 \<le> n2"
+    by simp
+  hence
+      "\<exists>c'. \<exists>s'. small_step_count (c,s) (c',s') (n1-n2)
+      \<and> small_step_count (c',s') (d,t) n2"
+    using
+      `n2 \<le> n1`
+      `small_step_count (c,s) (d,t) n1`
+      local.Suc.IH
+    by simp
+  then obtain c' s' where
+      "small_step_count (c,s) (c',s') (n1-n2)
+      \<and> small_step_count (c',s') (d,t) n2"
+    by auto
+  hence
+      "small_step_count (c,s) (c',s') (n1-n2)"
+      "small_step_count (c',s') (d,t) n2"
+    by auto
+  have "n1 - n2 \<ge> 1"
+    using
+      `n2 < n1`
+    by simp
+  hence
+      "\<exists>c''. \<exists>s''.
+      small_step_count (c,s) (c'',s'') (n1-n2-1)
+      \<and> small_step_count (c'',s'') (c',s') 1"
+    using
+      count_penult_step
+      `small_step_count (c,s) (c',s') (n1-n2)`
+    by blast
+  then obtain c'' s'' where
+      "small_step_count (c,s) (c'',s'') (n1-n2-1)
+      \<and> small_step_count (c'',s'') (c',s') 1"
+    by auto
+  hence
+      "small_step_count (c,s) (c'',s'') (n1-n2-1)"
+      "small_step_count (c'',s'') (c',s') 1"
+    by auto
+  hence "small_step_count (c'',s'') (d,t) (n2+1)"
+    using
+      `small_step_count (c',s') (d,t) n2`
+      `n2 \<ge> 0`
+      zero_count_same
+      small_step_count.Following
+    by (metis
+        add.commute
+        add.right_neutral
+        less_add_same_cancel1
+        order_le_less)
+  hence "small_step_count (c'',s'') (d,t) (Suc n2)"
+    by simp
+  have "(n1-n2-1) = (n1-(Suc n2))"
+    by simp
+  hence
+      "small_step_count (c,s) (c'',s'') (n1-(Suc n2))
+      \<and> small_step_count (c'',s'') (d,t) (Suc n2)"
+    using
+      `small_step_count (c'',s'') (d,t) (Suc n2)`
+      `small_step_count (c,s) (c'',s'') (n1-n2-1)`
+    by presburger
+  hence
+      "\<exists>c'. \<exists>s'.
+      small_step_count (c,s) (c',s') (n1-(Suc n2))
+      \<and> small_step_count (c',s') (d,t) (Suc n2)"
+    by auto
+  thus ?case
+    by simp
+qed
+
+lemma determ_trace_triangle:
+    "((c,s) \<rightarrow>* (d1,t1) \<and> (c,s) \<rightarrow>* (d2,t2))
+    \<longrightarrow> ((d1,t1) \<rightarrow>* (d2,t2) \<or> (d2,t2) \<rightarrow>* (d1,t1))"
+proof
+  assume "(c,s) \<rightarrow>* (d1,t1) \<and> (c,s) \<rightarrow>* (d2,t2)"
+  then obtain n1 n2 where
+      "small_step_count (c,s) (d1,t1) n1"
+      "small_step_count (c,s) (d2,t2) n2"
+    using leads_to_count
+    by presburger
+  have "n1 = n2 \<or> n1 > n2 \<or> n1 < n2"
+    by auto
+  thus "(d1,t1) \<rightarrow>* (d2,t2) \<or> (d2,t2) \<rightarrow>* (d1,t1)"
+  proof (elim disjE)
+    assume "n1 = n2"
+    hence "(d1,t1) = (d2,t2)"
+      using
+        `small_step_count (c,s) (d1,t1) n1`
+        `small_step_count (c,s) (d2,t2) n2`
+        equiv_count_impl_equiv_state
+      by presburger
+    hence "(d1,t1) \<rightarrow>* (d2,t2)"
+      by simp
+    thus "(d1,t1) \<rightarrow>* (d2,t2) \<or> (d2,t2) \<rightarrow>* (d1,t1)"
+      by (rule HOL.disjI1)
+  next
+    assume "n1 > n2"
+    hence "n1-(n1-n2) = n2"
+      by simp
+    have "n1-n2 >= 0"
+      by simp
+    have "n1 \<ge> (n1-n2)"
+      by simp
+    hence
+        "\<exists>c'. \<exists>s'.
+        small_step_count (c,s) (c',s') n2
+        \<and> small_step_count (c',s') (d1,t1) (n1-n2)"
+      using
+        `n1-(n1-n2) = n2`
+        `(n1-n2) \<ge> 0`
+        `small_step_count (c,s) (d1,t1) n1`
+        small_step_count_split
+      by metis
+    then obtain c' s' where
+        "small_step_count (c,s) (c',s') n2
+        \<and> small_step_count (c',s') (d1,t1) (n1-n2)"
+      by auto
+    hence
+        "small_step_count (c,s) (c',s') n2"
+        "small_step_count (c',s') (d1,t1) (n1-n2)"
+      by auto
+    hence "(c',s') = (d2,t2)"
+      using
+        equiv_count_impl_equiv_state
+        `small_step_count (c,s) (d2,t2) n2`
+      by simp
+    hence "small_step_count (d2,t2) (d1,t1) (n1-n2)"
+      using `small_step_count (c',s') (d1,t1) (n1-n2)`
+      by simp
+    hence "(d2,t2) \<rightarrow>* (d1,t1)"
+      using count_leads_to
+      by blast
+    thus ?thesis
+      by simp
+  next
+    assume "n1 < n2"
+    hence "n2-(n2-n1) = n1"
+      by simp
+    have "n2-n1 >= 0"
+      by simp
+    have "n2 \<ge> (n2-n1)"
+      by simp
+    hence
+        "\<exists>c'. \<exists>s'.
+        small_step_count (c,s) (c',s') n1
+        \<and> small_step_count (c',s') (d2,t2) (n2-n1)"
+      using
+        `n2-(n2-n1) = n1`
+        `(n2-n1) \<ge> 0`
+        `small_step_count (c,s) (d2,t2) n2`
+        small_step_count_split
+      by metis
+    then obtain c' s' where
+        "small_step_count (c,s) (c',s') n1
+        \<and> small_step_count (c',s') (d2,t2) (n2-n1)"
+      by auto
+    hence
+        "small_step_count (c,s) (c',s') n1"
+        "small_step_count (c',s') (d2,t2) (n2-n1)"
+      by auto
+    hence "(c',s') = (d1,t1)"
+      using
+        equiv_count_impl_equiv_state
+        `small_step_count (c,s) (d1,t1) n1`
+      by simp
+    hence "small_step_count (d1,t1) (d2,t2) (n2-n1)"
+      using `small_step_count (c',s') (d2,t2) (n2-n1)`
+      by simp
+    hence "(d1,t1) \<rightarrow>* (d2,t2)"
+      using count_leads_to
+      by blast
+    thus ?thesis
+      by simp
+  qed
+qed
+
+inductive state_changes ::
+    "com \<times> state \<Rightarrow> com \<times> state \<Rightarrow> nat \<Rightarrow> bool"
+  where
+None:
+  "state_changes (c,s) (c,s) 0" |
+Stateless:
+  "state_changes (c',s) (d,t) n
+   \<and> (c,s) \<rightarrow> (c',s)
+  \<Longrightarrow> state_changes (c,s) (d,t) n" |
+Stateful:
+  "state_changes (c',s') (d,t) n
+   \<and> (c,s) \<rightarrow> (c',s')
+   \<and> s \<noteq> s'
+  \<Longrightarrow> state_changes (c,s) (d,t) (n+1)"
+
+lemma state_change_count_exists:
+    "(c,s) \<rightarrow>* (d,t) \<Longrightarrow> \<exists>n. state_changes (c,s) (d,t) n"
+proof (induction rule: star_induct)
+  case (refl c s)
+  hence "state_changes (c,s) (c,s) 0"
+    by (rule state_changes.None)
+  thus "\<exists>n. state_changes (c,s) (c,s) n"
+    by (rule HOL.exI)
+next
+  case (step c s c' s' d t)
+  hence
+      "(c,s) \<rightarrow> (c',s')"
+      "\<exists>n. state_changes (c',s') (d,t) n"
+    by auto
+  then obtain n where
+      "state_changes (c',s') (d,t) n"
+    by auto
+  have "s = s' \<or> s \<noteq> s'"
+    by simp
+  thus "\<exists>n. state_changes (c,s) (d,t) n"
+  proof (elim disjE)
+    assume "s = s'"
+    hence "state_changes (c,s) (d,t) n"
+      using
+        state_changes.Stateless
+        `state_changes (c',s') (d,t) n`
+        `(c,s) \<rightarrow> (c',s')`
+      by blast
+    thus "\<exists>n. state_changes (c,s) (d,t) n"
+      by (rule HOL.exI)
+  next
+    assume "s \<noteq> s'"
+    hence "state_changes (c,s) (d,t) (n+1)"
+      using
+        state_changes.Stateful
+        `state_changes (c',s') (d,t) n`
+        `(c,s) \<rightarrow> (c',s')`
+      by blast
+    thus "\<exists>n. state_changes (c,s) (d,t) n"
+      by (rule HOL.exI)
+  qed
+qed
+
+lemma state_change_count_impl_leads_to:
+    "state_changes (c,s) (d,t) n \<Longrightarrow> (c,s) \<rightarrow>* (d,t)"
+proof (induction rule: state_changes.induct)
+  case (None c s)
+  thus "(c,s) \<rightarrow>* (c,s)"
+    by (rule star.refl)
+next
+  case (Stateless c' s d t n c)
+  hence
+      "(c',s) \<rightarrow>* (d,t)"
+      "(c,s) \<rightarrow> (c',s)"
+    by simp+
+  thus "(c,s) \<rightarrow>* (d,t)"
+    using star.step[of small_step]
+    by simp
+next
+  case (Stateful c' s' d t n c s)
+  hence
+      "(c',s') \<rightarrow>* (d,t)"
+      "(c,s) \<rightarrow> (c',s')"
+    by simp+
+  thus "(c,s) \<rightarrow>* (d,t)"
+    using star.step[of small_step]
+    by simp
+qed
+
+
+lemma leads_to_state_changes:
+    "(c,s) \<rightarrow>* (d,t) = (\<exists>n. state_changes (c,s) (d,t) n)"
+  using
+    state_change_count_impl_leads_to
+    state_change_count_exists
+  by blast
+
+lemma state_change_count_prepend_ge:
+    "state_changes (c',s') (d,t) n \<and> (c,s) \<rightarrow> (c',s')
+    \<Longrightarrow> \<exists>n'. state_changes (c,s) (d,t) n' \<and> n' \<ge> n"
+  using
+    state_changes.Stateful
+    state_changes.Stateless
+  by (metis dual_order.eq_iff le_add1)
+
+lemma zero_state_changes_impl_same:
+    "state_changes (c,s) (d,t) 0 \<Longrightarrow> s = t"
+proof -
+  assume "state_changes (c,s) (d,t) 0"
+  then obtain n where
+      "state_changes (c,s) (d,t) n"
+      "n = 0"
+    by auto
+  thus "s = t"
+  proof (induction "(c,s)" "(d,t)" n
+         arbitrary: c d
+         rule: state_changes.induct)
+    case None
+    thus "s = t"
+      by simp
+  next
+    case (Stateless c' d n c)
+    thus "s = t"
+      by simp
+  next
+    case (Stateful c' s' d n c)
+    thus "s = t" by simp
+  qed
+qed
+
+corollary zero_state_changes_is_same:
+    "(\<exists>d. state_changes (c,s) (d,t) 0) \<longleftrightarrow> (s = t)"
+proof
+  assume "\<exists>d. state_changes (c,s) (d,t) 0"
+  thus "s = t"
+    using zero_state_changes_impl_same
+    by blast
+next
+  assume "s = t"
+  hence "state_changes (c,s) (c,t) 0"
+    using state_changes.None
+    by simp
+  thus "\<exists>d. state_changes (c,s) (d,t) 0"
+    by (rule HOL.exI)
+qed
+
+lemma nonzero_state_changes_impl_interior_change:
+    "state_changes (c,s) (d,t) n \<and> n > 0
+    \<Longrightarrow> \<exists>c'. \<exists>s'.
+        (c,s) \<rightarrow>* (c',s')
+        \<and> (c',s') \<rightarrow>* (d,t)
+        \<and> s \<noteq> s'"
+proof -
+  assume "state_changes (c,s) (d,t) n \<and> n > 0"
+  hence
+      "state_changes (c,s) (d,t) n"
+      "n > 0"
+    by auto
+  thus
+      "\<exists>c'. \<exists>s'.
+      (c,s) \<rightarrow>* (c',s')
+      \<and> (c',s') \<rightarrow>* (d,t)
+      \<and> s \<noteq> s'"
+  proof (induction "(c,s)" "(d,t)" n
+         arbitrary: c d t
+         rule: state_changes.induct)
+    case None
+    thus ?case
+      by simp
+  next
+    case (Stateless c' d t n c)
+    thus ?case
+      by (metis star.step)
+  next
+    case (Stateful c' s' d t n c)
+    hence
+        "state_changes (c',s') (d,t) n"
+        "(c,s) \<rightarrow> (c',s')"
+        "s \<noteq> s'"
+      by simp+
+    hence "(c',s') \<rightarrow>* (d,t)"
+      using state_change_count_impl_leads_to
+      by simp
+    have "(c,s) \<rightarrow>* (c',s')"
+      using `(c,s) \<rightarrow> (c',s')`
+      by simp
+    hence
+        "(c,s) \<rightarrow>* (c',s')
+        \<and> (c',s') \<rightarrow>* (d,t)
+        \<and> s \<noteq> s'"
+      using
+        `(c',s') \<rightarrow>* (d,t)`
+        `s \<noteq> s'`
+      by simp
+    thus
+        "\<exists>c'. \<exists>s'.
+        (c,s) \<rightarrow>* (c',s')
+        \<and> (c',s') \<rightarrow>* (d,t)
+        \<and> s \<noteq> s'"
+      by auto
+  qed
+qed
+
+lemma non_ident_zero_state_change_impl_stateless:
+    "state_changes (c,s) (d,t) 0 \<and> c \<noteq> d
+    \<Longrightarrow> \<exists>c'. (c,s) \<rightarrow> (c',s)
+        \<and> state_changes (c',s) (d,t) 0"
+proof -
+  assume "state_changes (c,s) (d,t) 0 \<and> c \<noteq> d"
+  hence
+      "state_changes (c,s) (d,t) 0"
+      "c \<noteq> d"
+    by simp+
+  hence "(c,s) \<rightarrow>* (d,t)"
+    using state_change_count_impl_leads_to
+    by simp
+  have "s = t"
+    using `state_changes (c,s) (d,t) 0`
+    by (rule zero_state_changes_impl_same)
+  hence "(c,s) \<rightarrow>* (d,s)"
+    using `(c,s) \<rightarrow>* (d,t)`
+    by simp
+  hence "\<exists>c'. (c,s) \<rightarrow> (c',s) \<and> (c',s) \<rightarrow>* (d,s)"
+    using
+      `c \<noteq> d`
+      `state_changes (c,s) (d,t) 0`
+      imp_deterministic_small_step
+      star.cases
+      state_changes.simps
+    by (smt (verit)
+        Pair_inject
+        add_eq_0_iff_both_eq_0
+        one_neq_zero)
+  then obtain c' where
+      "(c,s) \<rightarrow> (c',s) \<and> (c',s) \<rightarrow>* (d,s)"
+    by (rule HOL.exE)
+  have "state_changes (c,s) (d,s) 0"
+    using
+      `state_changes (c,s) (d,t) 0`
+      `s = t`
+    by simp
+  hence "state_changes (c',s) (d,s) 0"
+  proof (cases rule: state_changes.cases)
+    case None
+    hence "c = d"
+      by simp
+    thus "state_changes (c',s) (d,s) 0"
+      using `c \<noteq> d`
+      by contradiction
+  next
+    case Stateless
+    thus "state_changes (c',s) (d,s) 0"
+      using
+        `(c,s) \<rightarrow> (c',s) \<and> (c',s) \<rightarrow>* (d,s)`
+        imp_deterministic_small_step
+      by blast
+  next
+    case (Stateful ct st nt)
+    hence
+        "nt+1 = 0
+        \<and> state_changes (ct,st) (d,s) nt
+        \<and>  (c,s) \<rightarrow> (ct,st)
+        \<and> s \<noteq> st"
+      by simp
+    hence "nt+1 = 0"
+      by simp
+    have "nt+1 > 0"
+      by simp
+    hence "nt+1 \<noteq> 0"
+      by simp
+    thus "state_changes (c',s) (d,s) 0"
+      using `nt+1 = 0`
+      by contradiction
+  qed
+  hence "state_changes (c',s) (d,t) 0"
+    using `s = t`
+    by simp
+  thus
+      "\<exists>c'. (c,s) \<rightarrow> (c',s)
+      \<and> state_changes (c',s) (d,t) 0"
+    using
+      `(c,s) \<rightarrow> (c',s) \<and> (c',s) \<rightarrow>* (d,s)`
+    by auto
+qed
+
+lemma state_change_count_append_ge:
+    "state_changes (c,s) (d',t') n \<and> (d',t') \<rightarrow> (d,t)
+    \<Longrightarrow> state_changes (c,s) (d,t) n' \<and> n' \<ge> n"
+proof -
+  assume
+      "state_changes (c,s) (d',t') n
+      \<and> (d',t') \<rightarrow> (d,t)"
+  hence 
+
+corollary non_ident_zero_state_changes_impl_last:
+    "state_changes (c,s) (d,t) 0 \<and> c \<noteq> d
+    \<Longrightarrow> \<exists>d'. state_changes (c,s) (d',t) 0
+        \<and> (d',t) \<rightarrow> (d,t)"
+proof -
+  assume "state_changes (c,s) (d,t) 0 \<and> c \<noteq> d"
+  hence
+      "state_changes (c,s) (d,t) 0"
+      "c \<noteq> d"
+    by simp+
+  hence "(c,s) \<rightarrow>* (d,t)"
+    using state_change_count_impl_leads_to
+    by simp
+  hence "star2 small_step (c,s) (d,t)"
+    by (rule star_impl_star2)
+  hence
+      "\<exists>d'. \<exists>t'.  star2 small_step (c,s) (d',t')
+      \<and> (d',t') \<rightarrow> (d,t)"
+  proof (cases rule: star2.cases)
+    case refl2
+    hence "c = d"
+      by simp
+    thus ?thesis
+      using `c \<noteq> d`
+      by contradiction
+  next
+    case (step2 y)
+    then obtain d' t' where
+        "star2 small_step (c,s) (d',t')"
+        "(d',t') \<rightarrow> (d,t)"
+      by (metis surj_pair)
+    thus
+        "\<exists>d'. \<exists>t'. star2 small_step (c,s) (d',t')
+        \<and> (d',t') \<rightarrow> (d,t)"
+      by auto
+  qed
+  hence "\<exists>d'. \<exists>t'. (c,s) \<rightarrow>* (d',t') \<and> (d',t') \<rightarrow> (d,t)"
+    using star2_impl_star
+    by metis
+  then obtain d' t' where
+      "(c,s) \<rightarrow>* (d',t') \<and> (d',t') \<rightarrow> (d,t)"
+    by auto
+  have "s = t"
+    using
+      `state_changes (c,s) (d,t) 0`
+      zero_state_changes_impl_same
+    by auto
+  have "t' = t"
+    sorry
+  hence "state_changes 
+
+
+
+
+lemma transitiv_zero_state_changes:
+    "state_changes (c,s) (c',s') 0
+    \<and> state_changes (c',s') (d,t) 0
+    \<Longrightarrow> state_changes (c,s) (d,t) 0"
+proof -
+  assume
+      "state_changes (c,s) (c',s') 0
+      \<and> state_changes (c',s') (d,t) 0"
+  hence
+      "state_changes (c,s) (c',s') 0"
+      "state_changes (c',s') (d,t) 0"
+    by simp+
+  hence
+      "s = s'"
+      "s' = t"
+    using zero_state_changes_impl_same
+    by simp+
+  hence "s = t"
+    by simp
+  have "(c,s) \<rightarrow>* (c',s')"
+    using `state_changes (c,s) (c',s') 0`
+    by (rule state_change_count_impl_leads_to)
+  hence "star2 small_step (c,s) (c',s')"
+    by (rule star_impl_star2)
+  thus "state_changes (c,s) (d,t) 0"
+  proof (induction "(c,s)" "(c',s')" rule: star2.induct)
+    case refl2
+    thus "state_changes (c,s) (d,t) 0"
+      using `state_changes (c',s') (d,t) 0`
+      by blast
+  next
+    case step2
+    then obtain c'' s'' where
+        "star2 small_step (c,s) (c'',s'')"
+        "(c'',s'') \<rightarrow> (c',s')"
+      by (metis surj_pair)
+    have "s'' = s' \<or> s'' \<noteq> s'"
+      by simp
+    thus "state_changes (c,s) (d,t) 0" sorry
+  qed
+qed
+
+
+lemma state_changes_transitivity:
+    "state_changes (c,s) (c',s') n1
+     \<and> state_changes (c',s') (d,t) n2
+    \<Longrightarrow> state_changes (c,s) (d,t) (n1+n2)"
+proof -
+  assume
+    "state_changes (c,s) (c',s') n1
+     \<and> state_changes (c',s') (d,t) n2"
+  thus "state_changes (c,s) (d,t) (n1+n2)"
+  proof (induction n2)
+    case 0
+    hence
+        "state_changes (c,s) (c',s') n1"
+        "state_changes (c',s') (d,t) 0"
+      by auto
+    hence "s' = t"
+      using zero_state_changes_impl_same
+      by simp
+    hence "state_changes (c,s) (c',t) n1"
+      using `state_changes (c,s) (c',s') n1`
+      by simp
+    thus "state_changes (c,s) (c',t) (n1+0)"
+      by simp
+  next
+    case (Suc n1)
+    then show ?case sorry
+  qed
+qed
+
+theorem determ_state_changes:
+    "state_changes (c,s) (d1,t1) n
+    \<and> state_changes (c,s) (d2,t2) n
+    \<Longrightarrow> t1 = t2"
+proof -
+  assume
+    "state_changes (c,s) (d1,t1) n
+    \<and> state_changes (c,s) (d2,t2) n"
+  thus "t1 = t2"
+  proof (induction n arbitrary: d1 t1 d2 t2)
+    case 0
+    hence "s = t1 \<and> s = t2"
+      using zero_state_changes_impl_same
+      by force
+    thus "t1 = t2"
+      by auto
+  next
+    case (Suc n)
+    fix d1' t1' d2' t2'
+    have
+        "state_changes (c,s) (d1',t1') n
+        \<and> state_changes (c,s) (d2',t2') n
+        \<Longrightarrow> t1' = t2'"
+      using local.Suc
+      by simp
+    thus "t1 = t2" sorry
+  qed
+qed
+
+(*
+lemma interior_changes_impl_nonzero_state_changes:
+    "(c,s) \<rightarrow>* (c',s') \<and> (c',s') \<rightarrow>* (d,t)
+    \<Longrightarrow> \<exists>n. \<exists>n'.
+        state_changes (c,s) (d,t) n
+        \<and> state_changes (c,s) (c',s') n'
+        \<and> n' \<le> n"
+proof -
+  assume "(c,s) \<rightarrow>* (c',s') \<and> (c',s') \<rightarrow>* (d,t)"
+  hence
+      "(c,s) \<rightarrow>* (c',s')"
+      "(c',s') \<rightarrow>* (d,t)"
+    by auto
+  hence "\<exists>n'. state_changes (c,s) (c',s') n'"
+    using state_change_count_exists
+    by simp
+  then obtain n' where
+      "state_changes (c,s) (c',s') n'"
+    by (rule HOL.exE)
+  have "\<exists>n''. state_changes (c',s') (d,t) n''"
+    using
+      `(c',s') \<rightarrow>* (d,t)`
+      state_change_count_exists
+    by simp
+  then obtain n'' where
+      "state_changes (c',s') (d,t) n''"
+    by (rule HOL.exE)
+  obtain n where
+      "n = n' + n''"
+    by simp
+  have "n'' \<ge> 0"
+    by simp
+  hence "n' \<le> n"
+    using `n = n' + n''`
+    by simp
+  have "state_changes (c,s) (d,t) n"
+    using
+      `n = n' + n''`
+      `state_changes (c,s) (c',s') n'`
+      `state_changes (c',s') (d,t) n''`
+    sorry
+*)
+
+lemma one_state_change_impl_diff_states:
+    "state_changes (c,s) (d,t) 1 \<Longrightarrow> s \<noteq> t"
+proof -
+  assume "state_changes (c,s) (d,t) 1"
+  then obtain n where
+      "state_changes (c,s) (d,t) n"
+      "n = 1"
+    by simp
+  thus "s \<noteq> t"
+  proof (induction "(c,s)" "(d,t)" n
+         arbitrary: c d
+         rule: state_changes.induct)
+    case None
+    hence "n = 0"
+      by simp
+    thus "s \<noteq> t"
+      using `n = 1`
+      by simp
+  next
+    case (Stateless c' d n c)
+    thus "s \<noteq> t"
+      by simp
+  next
+    case (Stateful c' s' d n c)
+    thus "s \<noteq> t"
+      using zero_state_changes_impl_same
+      by auto
+  qed
+qed
+
+(*
+theorem state_dist_le_step_count:
+    "small_step_count (c,s) (d,t) n
+    \<Longrightarrow> \<exists>n'. state_changes (c,s) (d,t) n' \<and> n' \<le> n"
+  sorry
+*)
+(*
+proof (induction "(c,s)" "(d,t)" n
+       rule: small_step_count.induct)
+  case Self
+  hence "state_changes (c,s) (d,t) 0"
+    using state_changes.None
+    by simp
+  have "0 \<le> n"
+    by simp
+  hence "\<exists>n'. state_changes (c,s) (d,t) n' \<and> n' \<le> n"
+    using `state_changes (c,s) (d,t) 0`
+    by auto
+  thus ?case
+    using `state_changes (c,s) (d,t) 0`
+    by blast
+next
+  case Step
+  hence "small_step_count (c,s) (d,t) 1"
+    by (rule small_step_count.Step)
+  have "s = t \<or> s \<noteq> t"
+    by simp
+  thus "\<exists>n'. state_changes (c,s) (d,t) n' \<and> n' \<le> 1"
+  proof (elim disjE)
+    assume "s = t"
+    hence "state_changes (c,s) (d,t) 0"
+      using
+        state_changes.None
+        state_changes.Stateless
+        local.Step
+      by blast
+    thus "\<exists>n'. state_changes (c,s) (d,t) n' \<and> n' \<le> 1"
+      using `state_changes (c,s) (d,t) 0`
+      by auto
+  next
+    assume "s \<noteq> t"
+    hence "state_changes (c,s) (d,t) 1"
+      using
+        state_changes.None
+        state_changes.Stateful
+        local.Step
+      by (metis One_nat_def add.commute plus_1_eq_Suc)
+    thus "\<exists>n'. state_changes (c,s) (d,t) n' \<and> n' \<le> 1"
+      by auto
+  qed
+next
+  case (Following n1 n2 c2 s2)
+  hence "\<exists>n'. state_changes (c,s) (c2,s2) n' \<and> n' \<le> n1" by try
+  thus "\<exists>n'. state_changes (c,s) (d,t) n' \<and> n' \<le> (n1+n2)"
+    by try
+qed
+  *)
+
+inductive finalish :: "(com \<times> state) \<Rightarrow> bool" where
+Final: "finalish (SKIP,s)" |
+ModuloParsing:
+    "finalish (c',s) \<and> (c,s) \<rightarrow> (c',s)
+    \<Longrightarrow> finalish (c,s)"
+
+theorem max_term_state_changes:
+    "(c,s) \<rightarrow>* (SKIP,f)
+    \<longleftrightarrow> (\<exists>x. \<forall>n. \<forall>d. \<forall>t.
+         state_changes (c,s) (d,t) n
+         \<longrightarrow> n \<le> x)"
+proof
+  assume "(c,s) \<rightarrow>* (SKIP,f)"
+  hence "\<exists>x. state_changes (c,s) (SKIP,f) x"
+    by (rule state_change_count_exists)
+  then obtain x where
+      "state_changes (c,s) (SKIP,f) x"
+    by (rule HOL.exE)
+  have
+      "\<not>(\<exists>n. \<exists>d. \<exists>t.
+      state_changes (c,s) (d,t) n
+      \<and> n > x)"
+  proof
+    assume
+        "\<exists>n. \<exists>d. \<exists>t. state_changes (c,s) (d,t) n \<and> n > x"
+    then obtain n d t where
+        "state_changes (c,s) (d,t) n \<and> n > x"
+      by auto
+    hence "(c,s) \<rightarrow>* (d,t)"
+      using state_change_count_impl_leads_to
+      by blast
+    hence "(d,t) \<rightarrow>* (SKIP,f) \<or> (SKIP,f) \<rightarrow>* (d,t)"
+      using
+        `(c,s) \<rightarrow>* (SKIP,f)`
+        determ_trace_triangle
+      by blast
+    thus False sorry
+  qed
+  thus
+      "\<exists>x. \<forall>n. \<forall>d. \<forall>t.
+      state_changes (c,s) (d,t) n
+      \<longrightarrow> n \<le> x"
+    sorry
+next
+  assume
+      "\<exists>x. \<forall>n. \<forall>d. \<forall>t.
+      state_changes (c,s) (d,t) n
+      \<longrightarrow> n \<le> x"
+  thus "(c,s) \<rightarrow>* (SKIP,f)"
+    sorry
+qed
+
+corollary skip_is_max_state_changes:
+    "(\<exists>f. state_changes (c,s) (SKIP,f) x)
+    \<longleftrightarrow> (\<forall>n. \<forall>d. \<forall>t.
+         state_changes (c,s) (d,t) n
+         \<longrightarrow> n \<le> x)"
+proof
+  assume "\<exists>f. state_changes (c,s) (SKIP,f) x"
+  then obtain f where
+      "state_changes (c,s) (SKIP,f) x"
+    by (rule HOL.exE)
+  have
+      "\<not>(\<exists>n. \<exists>d. \<exists>t.
+      state_changes (c,s) (d,t) n
+      \<and> n > x)"
+  proof
+    assume
+        "\<exists>n. \<exists>d. \<exists>t. state_changes (c,s) (d,t) n \<and> n > x"
+    then obtain n d t where
+        "state_changes (c,s) (d,t) n \<and> n > x"
+      by auto
+    hence "(c,s) \<rightarrow>* (d,t)"
+      using state_change_count_impl_leads_to
+      by blast
+    hence "(d,t) \<rightarrow>* (SKIP,f) \<or> (SKIP,f) \<rightarrow>* (d,t)"
+      using
+        `state_changes (c,s) (SKIP,f) x`
+        determ_trace_triangle
+        leads_to_state_changes
+      by blast
+    thus False
+      sorry
+  qed
+  thus
+      "\<forall>n. \<forall>d. \<forall>t.
+      state_changes (c,s) (d,t) n
+      \<longrightarrow> n \<le> x"
+    by fastforce
+next
+  assume
+      "\<forall>n. \<forall>d. \<forall>t.
+      state_changes (c,s) (d,t) n
+      \<longrightarrow> n \<le> x"
+  thus "\<exists>f. state_changes (c,s) (SKIP,f) x"
+    sorry
+qed
+
+theorem non_term_state_changes:
+    "\<not> final (c,s)
+    \<longleftrightarrow> (\<exists>d. \<exists>t. \<exists>n. state_changes (c,s) (d,t) n \<and> n > 0)"
+proof
+  assume "\<not> final (c,s)"
+  thus "\<exists>d. \<exists>t. \<exists>n. state_changes (c,s) (d,t) n \<and> n > 0"
+    sorry
+next
+  assume "\<exists>d. \<exists>t. \<exists>n. state_changes (c,s) (d,t) n \<and> n > 0"
+  thus "\<not> final (c,s)"
+    sorry
+qed
+
+(* Note that c1 \<sim> c2 would also be true for divergent
+   non-termination, so unfortunately we don't the
+   converse. *)
+theorem state_equiv_impl_big_step_equiv:
+    "\<forall>n. \<forall>t. (\<exists>d1. state_changes (c1,s) (d1,t) n)
+    = (\<exists>d2. state_changes (c2,s) (d2,t) n)
+    \<Longrightarrow> c1 \<sim> c2"
+proof -
+  assume assm:
+      "\<forall>n. \<forall>t. (\<exists>d1. state_changes (c1,s) (d1,t) n)
+      = (\<exists>d2. state_changes (c2,s) (d2,t) n)"
+  have
+      "(\<exists>f. (c1,s) \<rightarrow>* (SKIP,f))
+      \<or> \<not>(\<exists>f. (c1,s) \<rightarrow>* (SKIP,f))"
+    by auto
+  thus "c1 \<sim> c2"
+  proof (elim disjE)
+    assume "\<exists>f. (c1,s) \<rightarrow>* (SKIP,f)"
+    then obtain f where
+        "(c1,s) \<rightarrow>* (SKIP,f)"
+      by auto
+    hence "\<exists>x. state_changes (c1,s) (SKIP,f) x"
+      by (rule state_change_count_exists)
+    then obtain x where
+        "state_changes (c1,s) (SKIP,f) x"
+      by (rule HOL.exE)
+    hence
+        "\<not>(\<exists>x'. \<exists>d1'. \<exists>t1'.
+           state_changes (c1,s) (d1',t1') x'
+           \<and> x' > x)"
+      using skip_is_max_state_changes
+      by (metis not_less)
+    have
+        "\<not>(\<exists>x'. \<exists>d2'. \<exists>t2'.
+           state_changes (c2,s) (d2',t2') x'
+           \<and> x' > x)"
+    proof
+      assume
+          "\<exists>x'. \<exists>d2'. \<exists>t2'.
+          state_changes (c2,s) (d2',t2') x'
+          \<and> x' > x"
+      then obtain x' d2' t2' where
+          "state_changes (c2,s) (d2',t2') x'
+          \<and> x' > x"
+        by auto
+      hence
+          "\<exists>d1'. state_changes (c1,s) (d1',t2') x'
+          \<and> x' > x"
+        using assm
+        by blast
+      hence
+          "\<exists>x'. \<exists>d1'. \<exists>t1'.
+          state_changes (c1,s) (d1',t1') x'
+          \<and> x' > x"
+        by auto
+      thus False
+        using
+          `\<not>(\<exists>x'. \<exists>d1'. \<exists>t1'.
+             state_changes (c1,s) (d1',t1') x'
+             \<and> x' > x)`
+        by contradiction
+    qed
+    hence
+        "\<forall>n. \<forall>d2. \<forall>t2.
+        state_changes (c2,s) (d2,t2) n
+        \<longrightarrow> n \<le> x"
+      by fastforce
+    hence "(c2,s) \<rightarrow>* (SKIP,f)"
+      sorry
+    hence "(c2,s) \<Rightarrow> f"
+      by (rule small_term_impl_big_step)
+    thus "c1 \<sim> c2"
+      sorry
+  next
+    assume "\<not>(\<exists>f. (c1,s) \<rightarrow>* (SKIP,f))"
+    thus "c1 \<sim> c2"
+      sorry
+  qed
+qed
+
+theorem while_state_equiv_impl_big_step_equiv:
+    "(\<forall>s. \<not>final (c1,s) \<and> \<not>final (c2,s)
+      \<Longrightarrow> \<exists>t. \<exists>n. state_changes (c1,s) (c1,t) n
+          \<and> state_changes (c2,s) (c2,t) n
+          \<and> n > 0)
+    \<Longrightarrow> c1 \<sim> c2"
+proof -
+  assume
+    "\<forall>s. \<not>final (c1,s) \<and> \<not>final (c2,s)
+    \<Longrightarrow> \<exists>t. \<exists>n. state_changes (c1,s) (c1,t) n
+        \<and> state_changes (c2,s) (c2,t) n
+        \<and> n > 0"
+  thus "c1 \<sim> c2"
+    sorry
+qed
 
 end
