ch7/Exercise1mk2.thy
@@ -1,0 +1,54 @@
+theory Exercise1mk2
+  imports Sat
+begin
+
+fun srest :: "com \<Rightarrow> bexp \<Rightarrow> bexp" where
+"srest SKIP b = b" |
+"srest (v ::= a) b = (And b (VarEq v a))" |
+"srest (c1 ;; c2) b = b" |
+"srest (IF b1 THEN c1 ELSE c2) b2 = (
+
+fun rassigned :: "com \<Rightarrow> bexp \<Rightarrow> vname set" where
+"rassigned SKIP b = {}" |
+"rassigned (v ::= a) b = {v}" |
+"rassigned (c1 ;; c2) b
+  = (rassigned c1 b) \<union> (rassigned c2 (srest c1 b))" |
+"rassigned (IF b1 THEN c1 ELSE c2) b2
+  = (if (Sat (And b1 b2))
+      then (rassigned c1 (And b1 b2))
+      else {})
+    \<union> (if (Sat (And (Not b1) b2))
+        then (rassigned c2 (And (Not b1) b2))
+        else {})" |
+"rassigned (WHILE b1 DO c) b2
+  = (if (Sat (And b1 b2))
+      then (rassigned c (srest c (And b1 b2)))
+      else {})"
+
+(* NOTE: I did not notice the split_format behavior
+   until I saw it used by someone else to solve this
+   problem (i.e. https://github.com/kolya-vasiliev/concrete-semantics/blob/ae2a4b32ec63766e6a11e043d85d082c70eeaebc/Big_Step.thy#L68-L84),
+   but it is briefly documented in the Isar reference
+   manual. *)
+theorem not_assigned_oe_implies_unmodified:
+  "\<lbrakk> (c,s) \<Rightarrow> t; x \<notin> assigned_oe c \<rbrakk> \<Longrightarrow> s x = t x"
+  apply (induction rule: big_step.induct[split_format(complete)])
+        apply auto
+  done
+
+(* I tried creating a more accurate version of assigned
+   with the help of satisfiability of the guards seen
+   given all previous guards and assignments, but this
+   quickly became very complex. Furthermore, I have
+   heard on multiple occasions that variable assignment
+   and value reachability calculations are in general at
+   least uncomputable, and so overapproximations or
+   underapproximations are typically used instead (with
+   ongoing interest in particular overapproximation or
+   underapproximation formulations which could be more
+   valuable in the appropriate context). I admit to
+   having not seen the specific result myself, much less
+   explored the proof, but it does seem like the wrong
+   tree to be barking up in this introductory material.*)
+
+end
