ch7/Exercise5.thy
@@ -1,0 +1,104 @@
+theory Exercise5
+  imports IMP
+begin
+
+theorem if_conj:
+    "(IF (And b1 b2) THEN c1 ELSE c2)
+    \<sim> (IF b1 THEN (IF b2 THEN c1 ELSE c2) ELSE c2)"
+  (is "?LHS \<sim> ?RHS")
+proof -
+  have "(?RHS,s) \<Rightarrow> t" if assm: "(?LHS,s) \<Rightarrow> t" for s t
+  proof -
+    have "bval (And b1 b2) s \<or> \<not> bval (And b1 b2) s"
+      by simp
+    thus ?thesis
+    proof (elim disjE)
+      assume "bval (And b1 b2) s"
+      hence lsimp: "(?LHS,s) \<Rightarrow> t = (c1,s) \<Rightarrow>t" by auto
+      have "bval b1 s" and "bval b2 s"
+        using `bval (And b1 b2) s` by auto
+      hence "(?RHS,s) \<Rightarrow> t = (c1,s) \<Rightarrow> t" by auto
+      thus ?thesis using assm lsimp by auto
+    next
+      assume "\<not>bval (And b1 b2) s"
+      hence lsimp: "(?LHS,s) \<Rightarrow> t = (c2,s) \<Rightarrow> t" by auto
+      have "(\<not>bval b1 s) \<or> (\<not>bval b2 s)"
+        using `\<not>bval (And b1 b2) s` by simp
+      hence "(?RHS,s) \<Rightarrow> t = (c2,s) \<Rightarrow> t" by auto
+      thus ?thesis using assm lsimp by auto
+    qed
+  qed
+  moreover
+  have "(?LHS,s) \<Rightarrow> t" if assm: "(?RHS,s) \<Rightarrow> t" for s t
+  proof -
+    have "bval (And b1 b2) s \<or> \<not> bval (And b1 b2) s"
+      by simp
+    thus ?thesis
+    proof (elim disjE)
+      assume "bval (And b1 b2) s"
+      hence rsimp: "(?RHS,s) \<Rightarrow> t \<Longrightarrow> (c1,s) \<Rightarrow> t"
+        by auto
+      have "(?LHS,s) \<Rightarrow> t \<Longrightarrow> (c1,s) \<Rightarrow> t"
+        using `bval (And b1 b2) s` by auto
+      thus ?thesis using assm rsimp by auto
+    next
+      assume "\<not>bval (And b1 b2) s"
+      hence rsimp: "(?RHS,s) \<Rightarrow> t \<Longrightarrow> (c2,s) \<Rightarrow> t"
+        by auto
+      have "(?LHS,s) \<Rightarrow> t \<Longrightarrow> (c2,s) \<Rightarrow> t"
+        using `\<not>bval (And b1 b2) s` by auto
+      thus ?thesis using assm rsimp by auto
+    qed
+  qed
+  ultimately
+  show ?thesis by auto
+qed
+
+theorem while_conj:
+    "\<not>(\<forall>b1. \<forall>b2. \<forall>c.
+        (WHILE (And b1 b2) DO c)
+        \<sim> (WHILE b1 DO (WHILE b2 DO c)))"
+proof
+  assume spoz:
+      "\<forall>b1. \<forall>b2. \<forall>c.
+        (WHILE (And b1 b2) DO c)
+        \<sim> (WHILE b1 DO (WHILE b2 DO c))"
+  fix x
+  obtain l1 l2 ax x0 x1 x2 where witness:
+      "l1 = (Less (V x) (N 1))"
+      "l2 = (Less (V x) (N 2))"
+      "ax = (x ::= (Plus (V x) (N 1)))"
+      "x0 = (\<lambda>v.0::int)"
+      "x1 = x0(x:=1::int)"
+      "x2 = x0(x:=2::int)"
+    by simp
+  hence neq: "x1 \<noteq> x2"
+    by (smt (verit, del_insts) fun_upd_eqD)
+  have "(WHILE (And l1 l2) DO ax,x0) \<Rightarrow> x1" and
+      "(WHILE l1 DO (WHILE l2 DO ax),x0) \<Rightarrow> x2"
+    using witness by fastforce+
+  hence
+      "\<not>((WHILE (And l1 l2) DO ax)
+         \<sim> (WHILE l1 DO (WHILE l2 DO ax)))"
+    using diff_end_impl_diff_com neq by blast
+  thus False
+    using witness spoz by simp
+qed
+
+theorem while_disj:
+    "(WHILE (Or b1 b2) DO c)
+    \<sim> (WHILE (Or b1 b2) DO (c ;; WHILE b1 DO c))"
+  (is "?LHS \<sim> ?RHS")
+proof -
+  have
+      "\<forall>s. \<not>final (?LHS,s) \<or> \<not>final (?RHS,s)
+      \<Longrightarrow> \<exists>t. \<exists>n.
+      state_changes (?LHS,s) (?LHS,t) n
+      \<and> state_changes (?RHS,s) (?RHS,t) n
+      \<and> n > 0"
+    sorry
+  thus "?LHS \<sim> ?RHS"
+    by (rule while_state_equiv_impl_big_step_equiv)
+qed
+
+end
